src/Formalization/Examples/Example_Interval_Side_Proc_Global.thy
@@ -21,15 +21,14 @@ definition side_proc_global_ivl_s0 :: "ivl abs_state" where
 
 theorem proc_global_side_ivl_analysis:
   fixes s t :: store
-  assumes s_sound: "s \<in> ivl_domain.gamma_state side_proc_global_ivl_s0"
+  assumes s_sound: "s \<in> \<lbrakk>side_proc_global_ivl_s0\<rbrakk>"
   assumes runs: "cfg_runs_to inc_pi [''p''] (Call ''p'') s t"
   assumes side_solve_dom:
     "side_cfg_solve_dom_eff (compile_prog inc_pi [''p''] (Call ''p'')) ivl_etf bot
        side_proc_global_ivl_s0 ()
        (cfg_exit (compile_prog inc_pi [''p''] (Call ''p'')))"
-  shows "t \<in> ivl_domain.gamma_state
-       (side_analyse_eff inc_pi [''p''] (Call ''p'') ivl_etf bot side_proc_global_ivl_s0 ()
-         (cfg_exit (compile_prog inc_pi [''p''] (Call ''p''))))"
+  shows "t \<in> \<lbrakk>side_analyse_eff inc_pi [''p''] (Call ''p'') ivl_etf bot side_proc_global_ivl_s0 ()
+         (cfg_exit (compile_prog inc_pi [''p''] (Call ''p'')))\<rbrakk>"
 proof -
   have collect_exit:
     "t \<in> cfg_collect (compile_prog inc_pi [''p''] (Call ''p'')) {s}
