src/Formalization/Examples/Example_Side_Execute.thy
@@ -52,7 +52,7 @@ text \<open>
 
 corollary x1_certified_sound:
   "cfg_collect (prog_cfg x1_prog) cinit_stores (cfg_exit (prog_cfg x1_prog))
-   \<le> sign_domain.gamma_state (sign_exec_prog x1_prog)"
+   \<le> \<lbrakk>sign_exec_prog x1_prog\<rbrakk>"
   by (rule sign_exec_prog_sound_collecting[OF x1_terminates])
 
 subsection \<open>Annotated CFG visualisation\<close>
